Make basis build with two-argument FFI calls
Nothing fancy; will revisit later to actually use the added argument.

basis/basis_ffi.c
@@ -3,18 +3,18 @@
 
 /* stdout */
 
-void ffiputChar (char* a) {
+void ffiputChar (char* c, char* a) {
   putchar(a[0]);
 }
 
 /* stderr */
-void ffiputChar_err(char* a, long len) {
+void ffiputChar_err(char* c, char* a, long len) {
   putc(a[0], stderr);
 }
 
 /* stdin */
 
-void ffigetChar (char* a) {
+void ffigetChar (char* conf, char* a) {
   int c = getchar();
   if(c == EOF) {
     a[1] = 1;
@@ -32,7 +32,7 @@ extern char **argv;
 
 #define MAXLEN 256
 
-void ffigetArgs (char *a) {
+void ffigetArgs (char* c, char *a) {
         int i, j, k;
 
         for (i = 0, k = 0; (i < argc) && (k < MAXLEN); i++, k++) {
@@ -54,7 +54,7 @@ int nextFD() {
   return fd;
 }
 
-void ffiopen (char *a) {
+void ffiopen (char* c, char *a) {
   int fd = nextFD();
   if (fd < 255 && (infds[fd] = fopen(a,"r")))
     a[0] = fd;
@@ -62,15 +62,15 @@ void ffiopen (char *a) {
     a[0] = 255;
 }
 
-void ffifgetc (char *a) {
-  int c; /* not char, other EOF is mapped to a valid char */
+void ffifgetc (char* conf, char *a) {
+  int c; /* not char, otherwise EOF is mapped to a valid char */
   if (infds[a[0]] && (c = fgetc(infds[a[0]])) != EOF)
     a[0] = c;
   else
     a[0] = 255;
 }
 
-void fficlose (char *a) {
+void fficlose (char* conf, char *a) {
   if (infds[a[0]] && fclose(infds[a[0]]) == 0) {
     infds[a[0]] = NULL;
     a[0] = 1;
@@ -79,8 +79,8 @@ void fficlose (char *a) {
     a[0] = 0;
 }
 
-void ffiisEof (char *a) {
-  int c; /* not char, other EOF is mapped to a valid char */
+void ffiisEof (char* conf, char *a) {
+  int c; /* not char, otherwise EOF is mapped to a valid char */
   if (infds[a[0]])
     if ((c = fgetc(infds[a[0]])) == EOF)
       a[0] = 1;
