basis/stdinFFIScript.sml
@@ -4,14 +4,14 @@ open preamble
 val _ = new_theory"stdinFFI";
 
 val ffi_getChar_def = Define`
-  ffi_getChar (bytes:word8 list) inp =
+  ffi_getChar (conf:word8 list) (bytes:word8 list) inp =
     case(bytes, inp) of
     | ([b;f], "") => SOME ([b; 1w], "")
     | ([b;f], h::t) => SOME ([n2w (ORD h); 0w], t)
     | _ => NONE`
 
 val ffi_getChar_length = Q.store_thm("ffi_getChar_length",
-  `ffi_getChar bytes inp = SOME (bytes',inp') ⇒ LENGTH bytes' = LENGTH bytes`,
+  `ffi_getChar conf bytes inp = SOME (bytes',inp') ⇒ LENGTH bytes' = LENGTH bytes`,
   EVAL_TAC \\ every_case_tac \\ fs[]
   \\ Cases_on`bytes` \\ fs[NULL_EQ] \\ rw[] \\ rw[]
   \\ Cases_on`t` \\ fs[]);
