basis/stdoutFFIScript.sml
@@ -4,13 +4,13 @@ open preamble
 val _ = new_theory"stdoutFFI";
 
 val ffi_putChar_def = Define`
-  ffi_putChar (bytes:word8 list) out =
+  ffi_putChar (conf:word8 list) (bytes:word8 list) out =
     case(bytes, out) of
     | ([w], out) => SOME ([w], out ++ [CHR (w2n w)])
     | _ => NONE`
 
 val ffi_putChar_length = Q.store_thm("ffi_putChar_length",
-  `ffi_putChar bytes out = SOME (bytes',out') ⇒ LENGTH bytes' = LENGTH bytes`,
+  `ffi_putChar conf bytes out = SOME (bytes',out') ⇒ LENGTH bytes' = LENGTH bytes`,
   EVAL_TAC \\ every_case_tac \\ rw[] \\ Cases_on`bytes` \\ fs[NULL_EQ]
   \\ Cases_on`t` \\ fs[]);
 
